progress on proofs

src/sf_proof.v
@@ -2,6 +2,8 @@ Require sf_imp.
 Require sf_spec.
 Require Import RelDec.
 Require Import List.
+Require Import Sorted.
+Require Import Permutation.
 Import ListNotations.
 
 
@@ -247,14 +249,19 @@ Qed.
     
 Lemma no_viable_candidates_cons :
 forall a b e,
-sf_spec.no_viable_candidates candidate (e) (a ::  b) ->
-sf_spec.no_viable_candidates candidate e [a] /\
-sf_spec.no_viable_candidates candidate e b.
+sf_spec.no_viable_candidates candidate (e) (a ::  b) <->
+(sf_spec.no_viable_candidates candidate e [a] /\
+sf_spec.no_viable_candidates candidate e b).
+split.
 intros.
 unfold sf_spec.no_viable_candidates in *.
 split.
 intros. eapply H; eauto. inv H0; simpl in *; intuition.
 intros. eapply H; eauto. simpl. intuition.
+intros. intuition.
+unfold sf_spec.no_viable_candidates in *. simpl in *.
+intuition. eapply H0; eauto. 
+eapply H1; eauto.
 Qed.
 
 Lemma next_ranking_viable :
@@ -288,8 +295,9 @@ Lemma next_ranking_selected :
 forall bal cd bal' rec,
 sf_imp.next_ranking candidate _ rec bal = Some (cd, bal') ->
 sf_spec.selected_candidate candidate (in_record rec) bal cd.
+split.
 intros.
-unfold sf_spec.selected_candidate. split.
+unfold sf_spec.selected_candidate. 
 - unfold sf_spec.continuing_ballot. intro. 
   unfold sf_spec.exhausted_ballot in H0.
   destruct H0. 
@@ -302,8 +310,70 @@ unfold sf_spec.selected_candidate. split.
   inv H0. simpl in *. auto.
 Qed.
 
-  
+Lemma next_ranking_elimintaed :
+forall bal rec,
+sf_imp.next_ranking candidate _ rec bal = None ->
+sf_spec.exhausted_ballot candidate (in_record rec) bal.
+Proof.
+intros.
+unfold sf_spec.exhausted_ballot.
+induction bal.
+-  left. unfold sf_spec.no_viable_candidates. intros. inv H0.
+- simpl in *. destruct a.
+   + intuition. left. apply no_viable_candidates_cons. intuition.
+     unfold sf_spec.no_viable_candidates. intros. inv H0; intuition.
+     right. unfold sf_spec.overvote in *. destruct H1. exists x.
+     intuition. simpl. intuition.
+   + destruct (forallb (eq_dec c) a) eqn:?.
+     destruct (sf_imp.eliminated candidate reldec_candidate rec c) eqn:?; try congruence.
+     rewrite eliminated_correct in *.  
+     intuition. 
+     * left. unfold sf_spec.no_viable_candidates. intros. simpl in *. destruct H0.  
+       assert (candidate0 = c); subst; auto. rewrite forallb_forall in Heqb.
+       specialize (Heqb candidate0). simpl in H2. destruct H2; auto.
+       specialize (Heqb H0). apply reldec_correct_candidate in Heqb. auto.
+       unfold sf_spec.no_viable_candidates in *.
+       eapply H1; eauto.
+     * right. clear H Heqb0.
+       unfold sf_spec.overvote in *. 
+       destruct H1. intuition. destruct H1. destruct H. intuition.
+       exists x. simpl. intuition. left. intuition.
+       subst.
+       rewrite forallb_forall in Heqb. specialize (Heqb x0). 
+Admitted.
+ 
     
+Definition boolCmpToProp {A} (c : A -> A -> bool) :=
+fun a b => match c a b with
+           | true => True
+           | false => False
+end. 
+
+Lemma insert_sorted : forall {A} c sorted (a : A),
+    (forall a b, c a b = false -> c b a = true) ->
+    Sorted (boolCmpToProp c) sorted ->
+    Sorted (boolCmpToProp c) (sf_imp.insert c a sorted).
+induction sorted; intros. 
++ simpl. auto.
++ simpl. inv H0.
+  destruct (c a0 a) eqn:?. 
+  constructor. auto. constructor. unfold boolCmpToProp. rewrite Heqb. auto.
+  constructor. auto.  
+  specialize (IHsorted a0 H H3). 
+  destruct (sf_imp.insert c a0 sorted) eqn:?.
+Admitted. 
+  
+       
+Lemma insertion_sort_sorted' : forall {A} (l : list A) (sorted : list A) c,
+    (forall a b, c a b = false -> c b a = true) -> 
+    Sorted (boolCmpToProp c) sorted ->
+    Sorted (boolCmpToProp c) (sf_imp.insertionsort' c l sorted).   
+Proof.
+induction l.
++ intros. simpl. auto.
++ intros. simpl in *. apply IHl; auto.
+  apply insert_sorted; auto.
+Qed.      
 
 Lemma tabulate_continuing :
 forall rec elect res elect',
@@ -323,4 +393,439 @@ induction elect.
   
   unfold sf_imp.next_ranking in H.
 Admitted. 
+
+Locate Permutation.
+Print Permutation.
+
+Axiom insertionsort_permutation : forall A c (l: list A), Permutation (sf_imp.insertionsort c l) (l).
+
+Definition tb_func_to_Prop {c : Set} (f : list c -> option c) :=
+fun l cd => match f l with 
+         | Some x => x = cd
+         | None => False
+end.
+
+Lemma tabulate_correct : forall rec election rs election',
+sf_imp.tabulate candidate _ rec election = (rs, election') ->
+Forall (fun (x: (candidate * nat)) => let (cd, fc) := x in
+                 sf_spec.first_choices candidate (in_record rec) cd election fc) rs.
+Proof.
+intros.
+unfold sf_imp.tabulate in H. destruct (sf_imp.option_split
+             (map (sf_imp.next_ranking candidate reldec_candidate rec)
+                election)) eqn:?.
+induction election.
+- simpl in *. rewrite Forall_forall. intros. destruct x. inv Heqp. simpl in *. inv H.
+  simpl in *. inv H0.
+- simpl in Heqp. destruct (sf_imp.next_ranking candidate reldec_candidate rec a) eqn:?.
+  destruct p. destruct (sf_imp.option_split
+                (map (sf_imp.next_ranking candidate reldec_candidate rec)
+                   election)) eqn:?. inv Heqp. rewrite Forall_forall.
+  intros. destruct x. constructor.  
+  + admit.
+  + inv H.
+    pose proof (insertionsort_permutation _ (sf_imp.cnlt candidate) 
+                                          (sf_imp.tabulate' candidate reldec_candidate (Some c :: l1))).
+    eapply Permutation_in in H0; eauto.
+    unfold sf_imp.tabulate' in H0. simpl in H0.
+Admitted. 
+
+Lemma in_split : forall A B (f : A) (l : list (A * B)), 
+              In f (fst (split l)) -> 
+              exists n : B, In (f, n) l.
+Proof.
+induction l; intros.
+- simpl in *. inv H.
+- simpl in *. destruct a. simpl in *.
+  destruct (split l) eqn:?.
+  simpl in *. destruct H. 
+  + subst. eauto.
+  + intuition. destruct H0. eauto. 
+Qed.
+
+Lemma first_choices_app : 
+forall c l1 l2 x1 x2  r cnd, 
+sf_spec.first_choices c r cnd l1 x1 ->
+sf_spec.first_choices c r cnd l2 x2 ->
+sf_spec.first_choices c r cnd (l1 ++ l2) (x1 + x2).
+Proof.
+induction l1; intros.
+- simpl in *. inv H. simpl. auto.
+- simpl in *. Print sf_spec.first_choices.
+  inv H.
+  + apply sf_spec.first_choices_selected. auto. fold plus.
+    apply IHl1; auto.
+  + apply sf_spec.first_choices_not_selected; auto.
+Qed.
+
+Lemma first_choices_app_gt :
+forall c l1 l2 x1 x2 r cnd,
+sf_spec.first_choices c r cnd l1 x1 ->
+sf_spec.first_choices c r cnd (l1 ++ l2) (x2) ->
+x2 >= x1.
+Proof.
+induction l1; intros.
+- simpl in *. inv H. omega.
+- simpl in *. inv H; inv H0; try congruence; try omega.
+  eapply IHl1 in H5; eauto. omega.
+  eapply IHl1; eauto.
+Qed.
+
+Lemma first_choices_perm : 
+forall c l1 l2 x r cnd,
+Permutation l1 l2 ->
+sf_spec.first_choices c r cnd l1 x ->
+sf_spec.first_choices c r cnd l2 x.
+Proof.
+induction l1; intros.
+- apply Permutation_nil in H. subst. auto. 
+- assert (exists l2s l23, l2 = l2s ++ (a :: l23)). 
+  { eapply Permutation_in in H. instantiate (1 := a) in H.
+    apply List.in_split in H. auto.
+    constructor; auto. }
+  destruct H1. destruct H1.
+  subst.
+  apply Permutation_cons_app_inv in H.
+  inv H0.
+  + eapply (IHl1 _ n' r cnd) in H; auto.
+    clear - H H3.
+    { generalize dependent x1. generalize dependent n'.
+      induction x0; intros.
+      - simpl in *. constructor; auto.
+      - simpl in *. inv H. 
+        + constructor; auto.
+        + apply sf_spec.first_choices_not_selected; auto.
+    }
+  + eapply IHl1 in H; eauto.
+    { clear - H H3.
+      generalize dependent x1. generalize dependent x.
+      induction x0; intros.
+      - simpl in *. apply sf_spec.first_choices_not_selected; auto.
+      - simpl in *. inv H.
+        + constructor; auto.
+        + apply sf_spec.first_choices_not_selected; auto.
+    }
+Qed.
+
+Lemma rel_dec_refl : forall c, rel_dec c c = true.
+Proof.
+intros. apply rel_dec_correct. auto.
+Qed.
+
+Lemma increment_spec : forall m cd cds ct,
+cds = (fst (split m)) ->
+NoDup (cds) -> 
+(In (cd, ct) m -> In (cd, S ct) (sf_imp.increment candidate _ m cd)) /\
+(~In cd cds -> In (cd, 1) (sf_imp.increment candidate _ m cd)). 
+Proof.
+induction m; intros.
+- simpl in *. intuition.
+- simpl in *. destruct a. 
+  destruct (split m) eqn:?.
+  simpl in *. 
+  destruct (in_dec rel_dec_p cd cds). 
+  + subst.
+    split.
+    * { intros. simpl in *.
+        unfold eq_dec.
+        intuition.
+        - inv H2.  rewrite rel_dec_refl.
+          simpl. auto.
+        - subst. clear -Heqp H2 H0.
+          inv H0. assert (In cd l). apply in_split_l in H2. 
+          simpl in H2. rewrite Heqp in *. auto.
+          intuition.
+        - inv H2. inv H0. intuition.
+        - assert (c <> cd).
+          intro. subst. inv H0. intuition.
+          eapply rel_dec_neq_false in H.
+          rewrite H. simpl. right.
+          edestruct IHm. reflexivity.
+          inv H0; auto.
+          clear H4. auto. apply reldec_correct_candidate.
+      } 
+    * intuition.  
+  + subst. simpl in *. inv H0. unfold eq_dec.  
+    split. 
+      * { intuition.
+        - inv H0. intuition.
+        - eapply rel_dec_neq_false in H. rewrite H. 
+          edestruct IHm; eauto. simpl in *. auto.
+          apply reldec_correct_candidate.
+        }
+      * intuition. eapply rel_dec_neq_false in H4. rewrite H4.
+        simpl. 
+        edestruct IHm; eauto.
+        eapply reldec_correct_candidate.
+Grab Existential Variables. exact O.
+Qed.
+
+
+Lemma increment_not_0 : forall running cd,
+NoDup (fst (split running)) ->
+~In (cd, 0) (sf_imp.increment candidate reldec_candidate running cd).
+Proof.
+induction running; intros; intro.
+- unfold sf_imp.increment in *. simpl in *; intuition. congruence.
+- simpl in *. destruct a. destruct (eq_dec c cd) eqn:?.
+  + clear IHrunning. apply reldec_correct_candidate in Heqb. subst.
+    simpl in *. destruct (split running) eqn:?. simpl in *. 
+    inv H. intuition. congruence. apply in_split_l in H. 
+    simpl in H. rewrite Heqp in H. simpl. intuition.
+  + simpl in *. destruct (split running) eqn:?. simpl in *.
+    apply neg_rel_dec_correct in Heqb. destruct H0.
+    * inv H0. auto.
+    * inv H. intuition. eapply IHrunning; eauto.
+Qed.
+
+Lemma increment_nodup' : forall running cd c,
+~In c (fst (split running)) ->
+c <> cd ->
+~In c (fst (split (sf_imp.increment candidate reldec_candidate running cd))).
+Proof.
+induction running; intros.
+- simpl in *. intuition.
+- simpl in *.
+  destruct a. 
+  destruct (split running) eqn:?. simpl in H. intuition.
+  destruct (eq_dec c0 cd) eqn:?.
+  + simpl in *. rewrite Heqp in *. simpl in *. intuition.
+  + simpl in *. destruct (split
+                   (sf_imp.increment candidate reldec_candidate running cd)) eqn:?.
+    simpl in *. intuition. eapply IHrunning; eauto. 
+    rewrite Heqp0. simpl. auto.
+Qed.
+
+Lemma increment_nodup : forall running cd,
+NoDup (fst (split running)) -> 
+NoDup (fst (split (sf_imp.increment candidate reldec_candidate running cd))).
+induction running; intros.
+- simpl in *. constructor; auto. 
+- simpl in *. destruct a. destruct (eq_dec c cd) eqn:?.
+  + apply reldec_correct_candidate in Heqb. subst.
+    simpl in *.
+    destruct (split running) eqn:?. simpl in *. auto.
+  + simpl in *. destruct ( split (sf_imp.increment candidate reldec_candidate running cd)) eqn:?.
+    simpl.
+    destruct (split running) eqn:?. simpl in *. inv H.
+    eapply IHrunning in H3. instantiate (1:=cd) in H3. rewrite Heqp in H3.
+    simpl in H3. constructor; auto. intro. apply neg_rel_dec_correct in Heqb.
+    eapply increment_nodup'; eauto. instantiate (1:=running). 
+    rewrite Heqp0. simpl. auto.
+    rewrite Heqp. auto.
+Qed.    
+
+Lemma increment_neq : forall running c cd v,
+In (c, v) running ->
+c <> cd ->
+In (c, v) (sf_imp.increment candidate reldec_candidate running cd).
+Proof.
+induction running; intros.
+- inv H.
+- destruct a.
+  simpl in *.
+  destruct (eq_dec c0 cd) eqn:?.
+  + simpl in *. intuition.
+    apply reldec_correct_candidate in Heqb. inv H1. intuition.
+  + simpl in *. intuition.
+Qed.
+
+
+Lemma tabulate_not_0 : forall l cd v running,
+NoDup (fst (split running)) ->
+In (cd, v) running ->
+v <> 0 ->
+~In (cd, 0)
+   (sf_imp.tabulate'' candidate reldec_candidate l running).
+Proof.
+induction l; intros.
+- simpl in *. intuition. apply H1.
+  clear H1. induction running.
+  + inv H0.
+  + simpl in *. destruct a. destruct (split running) eqn:?. simpl in *.
+    intuition.
+    * inv H1. inv H0. auto.
+    * inv H1. inv H. intuition. apply in_split_l in H0. simpl in *.
+      rewrite Heqp in *. simpl in *. intuition.
+    * inv H. inv H0. apply in_split_l in H1. rewrite Heqp in *. simpl in *.
+      intuition.
+    * inv H. intuition.
+- simpl in *. destruct a. intro. intuition.
+  destruct (rel_dec_p c cd). 
+  + subst.
+    eapply IHl in H2; auto.
+    * apply increment_nodup. auto.
+    * instantiate (1:=S v). edestruct increment_spec. reflexivity.
+      apply H. apply H3. auto.
+    * intuition.
+  + eapply IHl in H2; auto.
+    * apply increment_nodup; auto.
+    * instantiate (1:=v). edestruct increment_spec. reflexivity.
+      apply H. apply increment_neq; auto.
+    * auto.
+  + eapply IHl in H0; auto.
+Grab Existential Variables. apply 0. apply c. (*ugh*)
+Qed.
+   
+  
+        
+Lemma tabulate''_first_choices : forall ef cd ct es running r
+(NODUP : NoDup (fst (split running))),
+In (cd, ct) (sf_imp.tabulate'' candidate _ 
+                               (fst (sf_imp.option_split
+                                      (map (sf_imp.next_ranking candidate reldec_candidate r)
+                                           ef))) running) -> 
+(forall cnd, ~In cnd (fst (split running)) -> sf_spec.first_choices candidate (in_record r) cnd es 0) ->
+Forall (fun x => let (cnd, n) := (x: candidate * nat) 
+                 in sf_spec.first_choices candidate (in_record r) cnd es n) running ->
+sf_spec.first_choices candidate (in_record r) cd (es ++ ef) ct. 
+Proof.
+induction ef; intros.
+- simpl in *. rewrite Forall_forall in *. specialize (H1 _ H). simpl in H1.
+  rewrite app_nil_r.  auto.
+- simpl in H. destruct (sf_imp.next_ranking candidate reldec_candidate r a) eqn:?.
+  +  destruct p. destruct (sf_imp.option_split
+                     (map (sf_imp.next_ranking candidate reldec_candidate r)
+                          ef)) eqn:?. simpl in *. 
+     assert (Permutation (a :: (es ++ ef)) (es ++ a :: ef)). 
+     apply Permutation_middle.
+     eapply first_choices_perm; eauto. clear H2.
+     apply next_ranking_selected in Heqo.
+     destruct (rel_dec_p c cd). 
+     * subst. destruct ct.
+       clear - H NODUP.
+       exfalso. 
+       eapply (tabulate_not_0 _ _ _ _ _ _ _ H).
+       constructor. auto. 
+       
+(*       destruct (in_dec _ (Some cd) (fst (sf_imp.option_split
+           (map (sf_imp.next_ranking candidate reldec_candidate r) ef)))). (map (sf_imp.next_ranking candidate _ r) (es ++ ef))).*)
+       eapply IHef; eauto.
+       rewrite Heqp. simpl. 
+       
+
+Lemma tab_inc_s : forall cd ct l running,
+NoDup (fst (split running)) ->
+In (cd, S ct)
+        (sf_imp.tabulate'' candidate reldec_candidate l
+           (sf_imp.increment candidate reldec_candidate running cd)) ->
+   In (cd, ct) (sf_imp.tabulate'' candidate reldec_candidate l running).
+Proof.
+induction l; intros.
++ simpl in *. 
+
+Lemma inc_spec_rev : forall running cd ct,
+In (cd, S ct) (sf_imp.increment candidate reldec_candidate running cd) ->
+In (cd, ct) running.
+Proof.
+induction running; intros.
+- simpl in *. intuition. inv H0.
+
+
+edestruct increment_spec; eauto.
+             
+edestruct increment_spec. Focus 3.
+         apply H0 in H.
+
+
+
+         apply increment_spec in H.
+         apply tabulate_spec in H.
+         simpl in *. unfold sf_imp.increment in H.
+          - unfold sf_imp.increment in *.
+            induction l. simpl in H. intuition. congruence.
+            apply IHl. simpl in H. destruct a0. destruct (eq_dec cd c).
+            apply IHl in H.
+         
+       
+       assert (l = fst (sf_imp.option_split
+         (map (sf_imp.next_ranking candidate reldec_candidate r) ef))). 
+       destruct ( sf_imp.option_split
+           (map (sf_imp.next_ranking candidate reldec_candidate r) ef)).
+       inv Heqp. auto.
+       subst. eapply IHef in H. 
+       rewrite app_comm_cons. apply H.
+       intros.
+       specialize (H0 cnd).
+       intuition. apply H0.  
+       { clear - H2.
+         induction running; auto.
+         simpl in *. destruct a. intros.
+         destruct (split running) eqn:?. simpl in *.
+         destruct H. 
+         subst. 
+         destruct (eq_dec cnd cd) eqn:?. simpl in *. rewrite Heqp in *. simpl in *.
+         auto. simpl in *. apply H2.
+         destruct (split (sf_imp.increment candidate reldec_candidate running cd)) eqn:?.
+         simpl. auto. apply IHrunning; auto.
+         destruct (eq_dec c cd). simpl in *. rewrite Heqp in *. simpl in *. intuition.
+         simpl in *. intros. apply H2.
+         destruct (split (sf_imp.increment candidate reldec_candidate running cd)).
+         simpl in *. auto.  }
+
+
+  +
+           
+                             
+
+apply sf_spec.first_choices_selected.
+       constructor; auto.
+           pose proof (first_choices_app _ _ (a::ef) _ (ct - x) _ _ H3).
+           cut (ct >= x). intros. 
+           rewrite <- Minus.le_plus_minus in H1; auto.
+           apply H1.
+           assert (ct >= x). eapply first_choices_app_gt; eauto.
+           apply H1.
+         SearchAbout app.
+         rewrite app_cons.
+         eapply first_choices_app.
+       
+
+
+
+    
+    
+
+       specialize (H1 (c, b)).
+  assert (sf_spec.first_choices candidate (in_record r) cd (es ++ ef) ct).
+  eapply IHef.
+ 
+  assert (l = fst (sf_imp.option_split
+         (map (sf_imp.next_ranking candidate reldec_candidate r) ef))). 
+  destruct ( sf_imp.option_split
+           (map (sf_imp.next_ranking candidate reldec_candidate r) ef)).
+  inv Heqp. auto. subst. eauto.
+  rewrite Forall_forall in *. intros.  
+  specialize (H0 (c, n)). apply H0. simpl in *.
+
+
+  
+  
+  
+ 
+
+forall b s, In b election ->
+                    continuing_ballot b ->
+                    In s (sf_imp.drop_none
+                            (map (sf_imp.next_ranking candidate reldec_candidate rec)
+                                 election)) ->  
+                    sf_spec.selected_candidate candidate (in_record rec) bal (fst x)).
+
+                                      
+
+Lemma run_election'_correct : forall fuel election winner tb rec rec',
+    sf_imp.run_election' candidate _ tb election rec fuel = (Some winner, rec') ->
+    sf_spec.winner candidate (tb_func_to_Prop tb) election (in_record []) winner.
+induction fuel; intros.
+simpl in *. congruence.
+Admitted.
+
+
+
+Theorem run_election_correct : forall election winner tb rec, 
+    sf_imp.run_election candidate _ tb election = (Some winner, rec) ->
+    sf_spec.winner candidate (tb_func_to_Prop tb) election (in_record []) winner.
+intros. unfold sf_imp.run_election in H. apply run_election'_correct in H. auto.
+Qed.
+
 
